Recognize more if-then-else statements that can be if-converted
Ignore debug statements that could have prevented the recognition
of a simple assignment.

Since debug statements can formally get stuck, revise the simulation
diagram to use the "eventually" modality.

backend/Selection.v
@@ -345,12 +345,17 @@ Inductive stmt_class : Type :=
   | SCassign (id: ident) (a: Cminor.expr)
   | SCother.
 
-Function classify_stmt (s: Cminor.stmt) : stmt_class :=
+Fixpoint classify_stmt (s: Cminor.stmt) : stmt_class :=
   match s with
   | Cminor.Sskip => SCskip
   | Cminor.Sassign id a => SCassign id a
-  | Cminor.Sseq Cminor.Sskip s => classify_stmt s
-  | Cminor.Sseq s Cminor.Sskip => classify_stmt s
+  | Cminor.Sbuiltin None (EF_debug _ _ _) _ => SCskip
+  | Cminor.Sseq s1 s2 =>
+      match classify_stmt s1, classify_stmt s2 with
+      | SCskip, c2 => c2
+      | c1, SCskip => c1
+      | _, _ => SCother
+      end
   | _ => SCother
   end.
 
